mailbox/verif_mailbox_specs.v
@@ -14,6 +14,10 @@ Instance CompSpecs_Preserve: change_composite_env verif_atomic_exchange.CompSpec
 Defined.
 Definition Vprog : varspecs. mk_varspecs prog. Defined.
 
+Definition extlink := ext_link_prog prog.
+Definition Espec := add_funspecs (Concurrent_Espec unit _ extlink) extlink Gprog.
+Existing Instance Espec.
+
 (* import funspecs from concurrency library *)
 Definition release_spec := DECLARE _release release_spec.
 Definition makelock_spec := DECLARE _makelock (makelock_spec _).
@@ -333,7 +337,7 @@ Definition writer_spec :=
 Definition main_spec :=
  DECLARE _main
   WITH gv: globals
-  PRE  [] main_pre prog [] gv
+  PRE  [] main_pre prog tt [] gv
   POST [ tint ] main_post prog [] gv.
 
 (* Create the environment containing all function specs. *)
