progs/verif_even.v
@@ -34,11 +34,8 @@ Qed.
 
 (* The Espec for odd is different from the Espec for even;
   the former has only "even" as an external function, and vice versa. *)
-Definition Espec := add_funspecs NullExtension.Espec (ext_link_prog even.prog) Gprog.
-Existing Instance Espec.
-
 Lemma prog_correct:
-  semax_prog prog Vprog Gprog.
+  semax_prog prog tt Vprog Gprog.
 Proof.
 prove_semax_prog.
 semax_func_cons_ext.
