progs/verif_funcptr.v
@@ -2,6 +2,7 @@ Require Import VST.floyd.proofauto.
 Require Import VST.progs.funcptr.
 Instance CompSpecs : compspecs. make_compspecs prog. Defined.
 Definition Vprog : varspecs. mk_varspecs prog. Defined.
+Existing Instance NullExtension.Espec.
 
 Local Open Scope Z.
 Local Open Scope logic.
@@ -21,7 +22,7 @@ Definition myfunc_spec := DECLARE _myfunc myspec.
 Definition main_spec :=
  DECLARE _main
   WITH gv : globals
-  PRE  [] main_pre prog nil gv
+  PRE  [] main_pre prog tt nil gv
   POST [ tint ] main_post prog nil gv.
 
 Definition Gprog : funspecs :=   ltac:(with_library prog [
