progs/verif_global.v
@@ -2,6 +2,7 @@ Require Import VST.floyd.proofauto.
 Require Import VST.progs.global.
 Instance CompSpecs : compspecs. make_compspecs prog. Defined.
 Definition Vprog : varspecs.  mk_varspecs prog. Defined.
+Existing Instance NullExtension.Espec.
 
 Definition h_spec :=
  DECLARE _h
@@ -17,7 +18,7 @@ Definition h_spec :=
 Definition main_spec :=
  DECLARE _main
   WITH gv: globals
-  PRE  [] main_pre prog [] gv
+  PRE  [] main_pre prog tt [] gv
   POST [ tint ] main_post prog [] gv.
 
 Definition Gprog : funspecs :=
