progs/verif_libglob.v
@@ -3,6 +3,7 @@ Require Import VST.progs.libglob.
 
 Instance CompSpecs : compspecs. make_compspecs prog. Defined.
 Definition Vprog : varspecs. mk_varspecs prog. Defined.
+Existing Instance NullExtension.Espec.
 
 Local Open Scope logic.
 
@@ -161,7 +162,7 @@ Definition client_spec :=
 Definition main_spec :=
   DECLARE _main
   WITH gv : globals
-  PRE  [] main_pre prog nil gv
+  PRE  [] main_pre prog tt nil gv
   POST [ tint ]  
      PROP() 
      LOCAL (temp ret_temp (Vint (Int.repr 5))) 
