progs/modular_queue.v
@@ -236,6 +236,7 @@ Definition module_fifo : module := {|
 |}.
 
 (***************************************************)
+Existing Instance NullExtension.Espec.
 
 Definition make_elem_spec :=
  DECLARE _make_elem
@@ -247,7 +248,7 @@ Definition make_elem_spec :=
 Definition main_spec :=
  DECLARE _main
   WITH u : unit
-  PRE  [] main_pre prog u
+  PRE  [] main_pre prog tt u
   POST [ tint ] main_post prog u.
 
 Definition Vprog : varspecs := nil.
@@ -264,8 +265,6 @@ Admitted.
 
 Lemma body_main:  semax_body Vprog Gtot f_main main_spec.
 Admitted.
-
-Existing Instance NullExtension.Espec.
 
 Lemma two_correct:
   semax_func Vprog Gtot
@@ -310,7 +309,7 @@ apply semax_func_nil.
 Qed.
 
 Lemma prog_correct:
-  semax_prog prog Vprog Gprog.
+  semax_prog prog tt Vprog Gprog.
 Proof.
 prove_semax_prog.
  next_module builtins_correct.
