progs/verif_insertion_sort.v
@@ -4,6 +4,7 @@ Require Import VST.progs.insertionsort.
 Require Import Sorted.
 Require Import Omega.
 Require Import Coq.Sorting.Permutation.
+Existing Instance NullExtension.Espec.
 
 Local Open Scope logic.
 
@@ -47,7 +48,7 @@ Definition insertionsort_spec :=
 Definition main_spec :=
  DECLARE _main
   WITH u : unit
-  PRE  [] main_pre prog u
+  PRE  [] main_pre prog tt u
   POST [ tint ] main_post prog u.
 
 Definition Vprog : varspecs := nil.
