progs/verif_logical_compare.v
@@ -3,6 +3,8 @@ Require Import VST.progs.logical_compare.
 Instance CompSpecs : compspecs.
 Proof. make_compspecs prog. Defined.
 
+Existing Instance NullExtension.Espec.
+
 (****  START *)
 
 Definition logical_and_result v1 v2 : int :=
@@ -102,7 +104,7 @@ Definition do_and_spec :=
 Definition main_spec :=
  DECLARE _main
   WITH gv: globals
-  PRE  [] main_pre prog nil gv
+  PRE  [] main_pre prog tt nil gv
   POST [ tint ] main_post prog nil gv.
 
 Definition Vprog : varspecs := nil.
@@ -139,10 +141,8 @@ start_function.
 forward.
 Qed.
 
-Existing Instance NullExtension.Espec.
-
 Lemma prog_correct:
-  semax_prog prog Vprog Gprog.
+  semax_prog prog tt Vprog Gprog.
 Proof.
 prove_semax_prog.
 semax_func_cons body_do_or.
