progs/verif_queue.v
@@ -7,6 +7,7 @@ Open Scope logic.
 
 Instance CompSpecs : compspecs. make_compspecs prog. Defined.
 Definition Vprog : varspecs. mk_varspecs prog. Defined.
+Existing Instance NullExtension.Espec.
 
 Definition t_struct_elem := Tstruct _elem noattr.
 Definition t_struct_fifo := Tstruct _fifo noattr.
@@ -326,7 +327,7 @@ Definition make_elem_spec :=
 Definition main_spec :=
  DECLARE _main
   WITH gv : globals
-  PRE  [] main_pre prog nil gv
+  PRE  [] main_pre prog tt nil gv
   POST [ tint ]
        PROP() LOCAL (temp ret_temp (Vint (Int.repr (1+10)))) SEP(TT).
 
@@ -564,10 +565,8 @@ forward_call (*  free(p, sizeof( *p)); *)
 forward. (* return i+j; *)
 Qed.
 
-Existing Instance NullExtension.Espec.
-
 Lemma prog_correct:
-  semax_prog prog Vprog Gprog.
+  semax_prog prog tt Vprog Gprog.
 Proof.
 prove_semax_prog. 
 semax_func_cons body_malloc. apply semax_func_cons_malloc_aux.
