progs/verif_queue2.v
@@ -7,6 +7,8 @@ Open Scope logic.
 
 Instance CompSpecs : compspecs. make_compspecs prog. Defined.
 Definition Vprog : varspecs. mk_varspecs prog. Defined.
+Existing Instance NullExtension.Espec.
+
 
 Definition t_struct_elem := Tstruct _elem noattr.
 Definition t_struct_fifo := Tstruct _fifo noattr.
@@ -122,7 +124,7 @@ Definition make_elem_spec :=
 Definition main_spec :=
  DECLARE _main
   WITH gv: globals
-  PRE  [] main_pre prog nil gv
+  PRE  [] main_pre prog tt nil gv
   POST [ tint ]
        PROP() LOCAL (temp ret_temp (Vint (Int.repr 1))) SEP(TT).
 
@@ -348,10 +350,8 @@ assert_PROP (isptr p3); [entailer! | rewrite if_false by (intro; subst; contradi
 forward. (* return i; *)
 Qed.
 
-Existing Instance NullExtension.Espec.
-
 Lemma prog_correct:
-  semax_prog prog Vprog Gprog.
+  semax_prog prog tt Vprog Gprog.
 Proof.
   prove_semax_prog.
   semax_func_cons body_malloc. apply semax_func_cons_malloc_aux.
