progs/verif_sumarray2.v
@@ -3,7 +3,7 @@ Require Import VST.progs.sumarray2. (* Import the AST of this C program *)
 (* The next line is "boilerplate", always required after importing an AST. *)
 Instance CompSpecs : compspecs. make_compspecs prog. Defined.
 Definition Vprog : varspecs.  mk_varspecs prog. Defined.
-
+Existing Instance NullExtension.Espec.
 
 (* Some definitions relating to the functional spec of this particular program.  *)
 Definition sum_Z : list Z -> Z := fold_right Z.add 0.
@@ -30,7 +30,7 @@ Definition sumarray_spec :=
 Definition main_spec :=
  DECLARE _main
   WITH gv: globals
-  PRE  [] main_pre prog nil gv
+  PRE  [] main_pre prog tt nil gv
   POST [ tint ]  
      PROP() 
      LOCAL (temp ret_temp (Vint (Int.repr (3+4)))) 
@@ -128,10 +128,8 @@ forward_call (*  s = sumarray(four+2,2); *)
   forward. (* return *)
 Qed.
 
-Existing Instance NullExtension.Espec.
-
 Lemma prog_correct:
-  semax_prog prog Vprog Gprog.
+  semax_prog prog tt Vprog Gprog.
 Proof.
 prove_semax_prog.
 semax_func_cons body_sumarray.
